Rename smart constructors for the Trace effect #137
Rename the smart constructors "Nil" and "LCons" for the Trace
effect to "NoMsg" and "Msg", respectively.
This should make their meaning clearer.

base/Free/Instance/Trace.v
@@ -16,13 +16,13 @@ Module Trace.
   (* Type synonym and smart constructors for the tracing effect. *)
   Module Import Monad.
     Definition Trace (A : Type) : Type := Free Shape Pos A.
-    Definition Nil {A : Type} 
+    Definition NoMsg {A : Type} 
                    (Shape' : Type) 
                    (Pos' : Shape' -> Type)
                    `{Injectable Shape Pos Shape' Pos'} 
                    (x : A) 
       : Free Shape' Pos' A := pure x.
-    Definition LCons {A : Type} 
+    Definition Msg {A : Type} 
                      (Shape' : Type) 
                      (Pos' : Shape' -> Type)
                      `{Injectable Shape Pos Shape' Pos'} 
@@ -86,7 +86,7 @@ Module Trace.
             nameMessages next n' scopes (pf tt)
           | impure (inr (inl (_,msg))) pf        =>
             let x := nameMessages (next + 1) scope scopes (pf tt) in
-            LCons (STrace Shape') (PTrace Pos') (Some (tripl scope next)) msg x
+            Msg (STrace Shape') (PTrace Pos') (Some (tripl scope next)) msg x
           | impure (inr (inr s)) pf              =>
             impure (inr s) (fun p => nameMessages next scope scopes (pf p)) 
           end
@@ -109,7 +109,7 @@ Module Trace.
   Instance Trace (Shape' : Type) (Pos' : Shape' -> Type)
                  `{I: Injectable Shape Pos Shape' Pos'}
    : Traceable Shape' Pos' := {
-     trace A msg p := @LCons A Shape' Pos' I None msg p
+     trace A msg p := @Msg A Shape' Pos' I None msg p
   }.
   (* There is no Partial instance. *)
 End Trace.
